erasure/theories/EWellformed.v
@@ -6,8 +6,7 @@ From MetaCoq.PCUIC Require Import PCUICAst PCUICAstUtils
      PCUICTyping PCUICInversion
      PCUICSafeLemmata. (* for welltyped *)
 From MetaCoq.SafeChecker Require Import PCUICWfEnvImpl.
-From MetaCoq.Erasure Require Import EAst EAstUtils EDeps EExtends
-    ELiftSubst ECSubst EWcbvEval EGlobalEnv.
+From MetaCoq.Erasure Require Import EAst EAstUtils ELiftSubst ECSubst EGlobalEnv.
 
 Local Open Scope string_scope.
 Set Asymmetric Patterns.
@@ -18,11 +17,119 @@ Set Equations Transparent.
 Local Set Keyed Unification.
 Require Import ssreflect ssrbool.
 
+Definition isSome {A} (o : option A) := 
+  match o with 
+  | None => false
+  | Some _ => true
+  end.
+
+Class ETermFlags := 
+  { has_tBox : bool
+  ; has_tRel : bool
+  ; has_tVar : bool
+  ; has_tEvar : bool
+  ; has_tLambda : bool
+  ; has_tLetIn : bool
+  ; has_tApp : bool
+  ; has_tConst : bool
+  ; has_tConstruct : bool
+  ; has_tCase : bool
+  ; has_tProj : bool
+  ; has_tFix : bool
+  ; has_tCoFix : bool
+  }.
+
+Class EEnvFlags := {
+  has_axioms : bool;
+  has_cstr_params : bool;
+  term_switches :> ETermFlags }.
+  
+Definition all_term_flags := 
+  {| has_tBox := true
+    ; has_tRel := true
+    ; has_tVar := true
+    ; has_tEvar := true
+    ; has_tLambda := true
+    ; has_tLetIn := true
+    ; has_tApp := true
+    ; has_tConst := true
+    ; has_tConstruct := true
+    ; has_tCase := true
+    ; has_tProj := true
+    ; has_tFix := true
+    ; has_tCoFix := true
+  |}.
+
+Definition all_env_flags := 
+  {| has_axioms := true; 
+     term_switches := all_term_flags;
+     has_cstr_params := true |}.
+    
+Section wf.
+  
+  Context {sw  : EEnvFlags}.
+  Variable Σ : global_context.
+
+  (* a term term is wellformed if
+    - it is closed up to k,
+    - it only contains constructos as indicated by sw,
+    - all occuring constructors are defined,
+    - all occuring constants are defined, and
+    - if has_axioms is false, all occuring constants have bodies *)
+  
+  Fixpoint wellformed k (t : term) : bool :=
+    match t with
+    | tRel i => has_tRel && Nat.ltb i k
+    | tEvar ev args => has_tEvar && List.forallb (wellformed k) args
+    | tLambda _ M => has_tLambda && wellformed (S k) M
+    | tApp u v => has_tApp && wellformed k u && wellformed k v
+    | tLetIn na b b' => has_tLetIn && wellformed k b && wellformed (S k) b'
+    | tCase ind c brs => has_tCase && 
+      let brs' := List.forallb (fun br => wellformed (#|br.1| + k) br.2) brs in
+      isSome (lookup_inductive Σ ind.1) && wellformed k c && brs'
+    | tProj p c => has_tProj && isSome (lookup_inductive Σ p.1.1) && wellformed k c
+    | tFix mfix idx => has_tFix &&
+      let k' := List.length mfix + k in
+      List.forallb (test_def (wellformed k')) mfix
+    | tCoFix mfix idx => has_tCoFix &&
+      let k' := List.length mfix + k in
+      List.forallb (test_def (wellformed k')) mfix
+    | tBox => has_tBox
+    | tConst kn => has_tConst && 
+      match lookup_constant Σ kn with
+      | Some d => has_axioms || isSome d.(cst_body)
+      | _ => false 
+      end
+    | tConstruct ind c => has_tConstruct && isSome (lookup_constructor Σ ind c)
+    | tVar _ => has_tVar
+    end.
+
+End wf.
+
+
+Definition wf_global_decl {sw : EEnvFlags} Σ d : bool :=
+  match d with
+  | ConstantDecl cb => option_default (fun b => wellformed Σ 0 b) cb.(cst_body) has_axioms
+  | InductiveDecl idecl => has_cstr_params || (idecl.(ind_npars) == 0)
+  end.
+
+Inductive wf_glob {efl : EEnvFlags} : global_declarations -> Prop :=
+| wf_glob_nil : wf_glob []
+| wf_glob_cons kn d Σ : 
+  wf_glob Σ ->
+  wf_global_decl Σ d ->
+  fresh_global kn Σ ->
+  wf_glob ((kn, d) :: Σ).
+Derive Signature for wf_glob.
+
+Implicit Types (efl : EEnvFlags).
+
 Section EEnvFlags.
   Context {efl : EEnvFlags}.
   Context {Σ : global_declarations}.
+  Notation wellformed := (wellformed Σ).
   
-  Lemma wellformed_closed {k t} : wellformed Σ k t -> closedn k t.
+  Lemma wellformed_closed {k t} : wellformed k t -> closedn k t.
   Proof.
     induction t in k |- * using EInduction.term_forall_list_ind; intros;
       simpl in * ; rewrite -> ?andb_and in *;
@@ -32,7 +139,7 @@ Section EEnvFlags.
         try solve [simpl lift; simpl closed; f_equal; auto; repeat (rtoProp; simpl in *; solve_all)]; try easy.
   Qed.
 
-  Lemma wellformed_up {k t} : wellformed Σ k t -> forall k', k <= k' -> wellformed Σ k' t.
+  Lemma wellformed_up {k t} : wellformed k t -> forall k', k <= k' -> wellformed k' t.
   Proof.
     induction t in k |- * using EInduction.term_forall_list_ind; intros;
       simpl in * ; rewrite -> ?andb_and in *;
@@ -43,7 +150,7 @@ Section EEnvFlags.
     eapply Nat.ltb_lt. now eapply Nat.ltb_lt in H2.
   Qed.
 
-  Lemma wellformed_lift n k k' t : wellformed Σ k t -> wellformed Σ (k + n) (lift n k' t).
+  Lemma wellformed_lift n k k' t : wellformed k t -> wellformed (k + n) (lift n k' t).
   Proof.
     revert k.
     induction t in n, k' |- * using EInduction.term_forall_list_ind; intros;
@@ -61,9 +168,9 @@ Section EEnvFlags.
   Qed.
 
   Lemma wellformed_subst_eq {s k k' t} {hast : has_tRel} :
-    forallb (wellformed Σ k) s -> 
-    wellformed Σ (k + k' + #|s|) t =
-    wellformed Σ (k + k') (subst s k' t).
+    forallb (wellformed k) s -> 
+    wellformed (k + k' + #|s|) t =
+    wellformed (k + k') (subst s k' t).
   Proof.
     intros Hs. solve_all. revert Hs.
     induction t in k' |- * using EInduction.term_forall_list_ind; intros;
@@ -107,8 +214,8 @@ Section EEnvFlags.
   Qed.
 
   Lemma wellformed_subst s k t {hast : has_tRel}: 
-    forallb (wellformed Σ k) s -> wellformed Σ (#|s| + k) t -> 
-    wellformed Σ k (subst0 s t).
+    forallb (wellformed k) s -> wellformed (#|s| + k) t -> 
+    wellformed k (subst0 s t).
   Proof.
     intros.
     unshelve epose proof (wellformed_subst_eq (k':=0) (t:=t) H); auto.
@@ -117,9 +224,9 @@ Section EEnvFlags.
   Qed.
 
   Lemma wellformed_csubst t k u {hast : has_tRel} : 
-    wellformed Σ 0 t -> 
-    wellformed Σ (S k) u -> 
-    wellformed Σ k (ECSubst.csubst t 0 u).
+    wellformed 0 t -> 
+    wellformed (S k) u -> 
+    wellformed k (ECSubst.csubst t 0 u).
   Proof.
     intros.
     rewrite ECSubst.closed_subst //.
@@ -129,9 +236,9 @@ Section EEnvFlags.
   Qed.
 
   Lemma wellformed_substl ts k u {hast : has_tRel}: 
-    forallb (wellformed Σ 0) ts -> 
-    wellformed Σ (#|ts| + k) u -> 
-    wellformed Σ k (ECSubst.substl ts u).
+    forallb (wellformed 0) ts -> 
+    wellformed (#|ts| + k) u -> 
+    wellformed k (ECSubst.substl ts u).
   Proof.
     induction ts in u |- *; cbn => //.
     move/andP=> [] cla clts.
@@ -139,4 +246,150 @@ Section EEnvFlags.
     eapply wellformed_csubst => //.
   Qed.
 
+  Lemma wellformed_fix_subst mfix {hast : has_tFix}: 
+    forallb (EAst.test_def (wellformed (#|mfix| + 0))) mfix ->
+    forallb (wellformed 0) (fix_subst mfix).
+  Proof.
+    solve_all.
+    unfold fix_subst.
+    move: #|mfix| => n.
+    induction n. constructor.
+    cbn. rewrite H IHn //. now rewrite hast.
+  Qed.
+
+  Lemma wellformed_cofix_subst mfix {hasco : has_tCoFix}: 
+    forallb (EAst.test_def (wellformed (#|mfix| + 0))) mfix ->
+    forallb (wellformed 0) (cofix_subst mfix).
+  Proof.
+    solve_all.
+    unfold cofix_subst.
+    move: #|mfix| => n.
+    induction n. constructor.
+    cbn. rewrite H IHn // hasco //.
+  Qed.
+
+  Lemma wellformed_cunfold_fix mfix idx n f {hast : has_tRel} : 
+    wellformed 0 (EAst.tFix mfix idx) ->
+    cunfold_fix mfix idx = Some (n, f) ->
+    wellformed 0 f.
+  Proof.
+    move=> cl.
+    rewrite /cunfold_fix.
+    destruct nth_error eqn:heq => //.
+    cbn in cl. move/andP: cl => [hastf cl].
+    have := (nth_error_forallb heq cl) => cld. 
+    move=> [=] _ <-.
+    eapply wellformed_substl => //. now eapply wellformed_fix_subst.
+    rewrite fix_subst_length.
+    apply cld.
+  Qed.
+
+  Lemma wellformed_cunfold_cofix mfix idx n f {hast : has_tRel} : 
+    wellformed 0 (EAst.tCoFix mfix idx) ->
+    cunfold_cofix mfix idx = Some (n, f) ->
+    wellformed 0 f.
+  Proof.
+    move=> cl.
+    rewrite /cunfold_cofix.
+    destruct nth_error eqn:heq => //.
+    cbn in cl. move/andP: cl => [hastf cl].
+    have := (nth_error_forallb heq cl) => cld. 
+    move=> [=] _ <-.
+    eapply wellformed_substl => //. now eapply wellformed_cofix_subst.
+    rewrite cofix_subst_length.
+    apply cld.
+  Qed.
+
+  Lemma wellformed_iota_red pars c args brs br {hast : has_tRel}:
+    forallb (wellformed 0) args ->
+    nth_error brs c = Some br ->
+    #|skipn pars args| = #|br.1| ->
+    wellformed #|br.1| br.2 ->
+    wellformed 0 (iota_red pars args br).
+  Proof.
+    intros clargs hnth hskip clbr.
+    rewrite /iota_red.
+    eapply wellformed_substl => //.
+    now rewrite forallb_rev forallb_skipn.
+    now rewrite List.rev_length hskip Nat.add_0_r.
+  Qed.
+
+  Lemma wellformed_iota_red_brs pars c args brs br {hast : has_tRel}:
+    forallb (wellformed 0) args ->
+    nth_error brs c = Some br ->
+    #|skipn pars args| = #|br.1| ->
+    forallb (fun br => wellformed (#|br.1| + 0) br.2) brs ->
+    wellformed 0 (iota_red pars args br).
+  Proof.
+    intros clargs hnth hskip clbr.
+    eapply wellformed_iota_red; tea => //.
+    eapply nth_error_forallb in clbr; tea.
+    now rewrite Nat.add_0_r in clbr.
+  Qed.
+
+  Lemma wellformed_mkApps n f args {hast : has_tApp} : wellformed n (mkApps f args) = wellformed n f && forallb (wellformed n) args.
+  Proof.
+    induction args using rev_ind; cbn; auto => //.
+    - now rewrite andb_true_r.
+    - now rewrite mkApps_app /= IHargs hast /= forallb_app /= // !andb_assoc andb_true_r.
+  Qed.
+
 End EEnvFlags.
+
+Lemma extends_lookup {efl} {Σ Σ' c decl} :
+  wf_glob Σ' ->
+  extends Σ Σ' ->
+  lookup_env Σ c = Some decl ->
+  lookup_env Σ' c = Some decl.
+Proof.
+  intros wfΣ' [Σ'' ->]. simpl.
+  induction Σ'' in wfΣ', c, decl |- *.
+  - simpl. auto.
+  - specialize (IHΣ'' c decl). forward IHΣ''.
+    + now inv wfΣ'.
+    + intros HΣ. specialize (IHΣ'' HΣ).
+      inv wfΣ'. simpl in *.
+      case: eqb_spec; intros e; subst; auto.
+      apply lookup_env_Some_fresh in IHΣ''; contradiction.
+Qed.
+
+Lemma extends_is_propositional {efl} {Σ Σ'} : 
+  wf_glob Σ' -> extends Σ Σ' ->
+  forall ind b, inductive_isprop_and_pars Σ ind = Some b -> inductive_isprop_and_pars Σ' ind = Some b.
+Proof.
+  intros wf ex ind b.
+  rewrite /inductive_isprop_and_pars.
+  destruct lookup_env eqn:lookup => //.
+  now rewrite (extends_lookup wf ex lookup).
+Qed.
+
+Lemma extends_wellformed {efl} {Σ Σ'} : 
+  wf_glob Σ' -> extends Σ Σ' ->
+  forall t n, wellformed Σ n t -> wellformed Σ' n t.
+Proof.
+  intros wf ex t.
+  induction t using EInduction.term_forall_list_ind; cbn => //; intros; rtoProp; intuition auto; solve_all.
+  all:destruct lookup_env eqn:hl => //; rewrite (extends_lookup wf ex hl).
+  all:destruct g => //.
+Qed.
+
+Lemma extends_wf_global_decl {efl} {Σ Σ'} : 
+  wf_glob Σ' -> extends Σ Σ' ->
+  forall t, wf_global_decl Σ t -> wf_global_decl Σ' t.
+Proof.
+  intros wf ex []; cbn => //.
+  destruct (cst_body c) => /= //.
+  now eapply extends_wellformed.
+Qed.
+
+Lemma lookup_env_wellformed {efl} {Σ kn decl} : wf_glob Σ -> 
+  EGlobalEnv.lookup_env Σ kn = Some decl -> wf_global_decl Σ decl.
+Proof.
+  induction Σ; cbn => //.
+  intros wf. depelim wf => /=.
+  destruct (eqb_spec kn kn0).
+  move=> [= <-]. eapply extends_wf_global_decl; tea. constructor; auto. now eexists [_].
+  intros hn.
+  eapply extends_wf_global_decl; tea. 3:eapply IHΣ => //.
+  now constructor. now eexists [_].
+Qed.
