erasure/theories/EExtends.v
@@ -1,7 +1,7 @@
 From Coq Require Import ssreflect.
 From Equations Require Import Equations.
 From MetaCoq.Template Require Import config utils Kernames.
-From MetaCoq.Erasure Require Import EGlobalEnv EAst Extract.
+From MetaCoq.Erasure Require Import EGlobalEnv EAst Extract EWellformed.
 
 Section EEnvFlags.
   Context (efl : EEnvFlags).
